Intermediate step. Changed the datatypes. Actor class is now a parameter of Actor. No longer a map. Avoids passing an extra parameter to functions involving actor class. The methods and lemmas are not yet changed to reflect this."

config.dfy
@@ -1,41 +1,42 @@
 ////////////////////CONFIG////////////////////
-datatype C = createConfig(heap: Heap, actors: Actors)
+datatype Config = createConfig(heap: Heap, actors: Actors)
 
 //Heap 
 datatype Heap = CHeap(objs: map<Addr, map<FId, Addr>>)
 
 //Addrs
-type Addr = int
-type ObjectAddr = int
-type ActorAddr = int 
+datatype Addr = OA(oa: ObjectAddr) | AA(aa: ActorAddr) | ERR
+type ObjectAddr = nat
+type ActorAddr = nat
 /* 
 datatype Addr = Cons(id: int)
 datatype ObjectAddr = Cons(id: int)
 datatype ActorAddr = Cons(id: int) 
 */
 
-type Actors = map<ActorAddr, Actor>
+//type Actors = map<ActorAddr, Actor>
+type Actors = seq<Actor>
 //datatype Queue = CQueue(msgs: seq<Msg>)
 type Queue = seq<Msg>
-datatype Msg = orca(i: Addr, z: int) | app(b: BId, is: seq<ObjectAddr>)
-//datatype Msg = orca(i: Addr, z: int) | app(f: Frame) ..alternative: only a frame is passed
+//datatype Msg = orca(i: Addr, z: int) | app(b: BId, is: seq<ObjectAddr>)
+datatype Msg = orca(i: Addr, z: int) | app(f: Frame) // ..alternative: only a frame is passed
 //type Actor = (q: Queue, rct: RefCountT, s: State)
-datatype Actor = CActor(q: Queue, rct: RefCountT, st: State)
+datatype Actor = CActor(q: Queue, rct: RefCountT, st: State, cl: ClassId)
 type RefCountT = map<Addr, int>
 
 //Paths 
-datatype LP = This | frm(zero: int, x: VarId) | cons(lp: LP, f: FId)
-datatype MP = frm(k: int, x: VarId) | cons(mp: MP, f: FId)
+datatype DP = This | LP(zero: int, x: VarId) | MP(k: int, x': VarId) | cons(dp: DP, f: FId)
 datatype SP = This | bsp(b: BId, x: VarId) | cons(sp: SP, f: FId)
-datatype Capability = WRITE | READ | TAG
+datatype Capability = WRITE | READ | TAG | ERR
 
 //State 
 datatype State = idl | exe(f: Frame) | snd(f': Frame, a: Actor, m: Msg, ws: Workset)
                 | mkU(ms: Marks) | trc(ms': Marks) | mkR(ms'': Marks) | cll(ms''': Marks)
-datatype Frame = CFrame(BId, map<VarId, Addr>)
+datatype Frame = CFrame(b: BId, Map: map<VarId, Addr>)
 type Workset = set<Addr> 
 //datatype Marks = CMarks(map<Addr, RU>)
 type Marks = map<Addr, RU>
+
 datatype RU = R | U
 
 //IDs
@@ -44,6 +45,95 @@ type BId = int
 type ClassId = int
 type VarId = int
 
+//type Class = map<ActorAddr, ClassId>
+/*
+//pass maps around?
+function sees(cl: Class, a: ActorAddr, sp: SP) : Capability
+{
+    if a in cl then sees'(cl[a], sp) else Capability.ERR
+}
+
+function sees'(cid: ClassId, sp: SP) : Capability
+
+lemma A1(c: Config, cl: Class, a: ActorAddr, sp: SP, f: FId, cappa: Capability) 
+requires sees(cl, a, SP.cons(sp, f)) == cappa //pass cappa as param instead?
+//requires sees(cl, c, a, SP.cons(sp, f)) == _ 
+ensures exists cappa' :: cappa' != TAG && sees(cl, a, sp) == cappa'
+
+lemma A2(c: Config, cl: Class, a: ActorAddr, sp: SP, f: FId) 
+requires sees(cl, a, SP.cons(sp, f)) == WRITE
+ensures sees(cl, a, sp) == WRITE
 
 
+/*
+function method C(a: ActorAddr, dp: DP, c: Config) : Addr 
+{
+    all_actors_in_config();
+    match dp 
+    case This => AA(a)
+    //case LP(zero, x) => if c.actors[a].st == exe(f: Frame) then {Capability.ERR} else {ERR}
+    case MP(k, x) => 
+        match c.actors[a].q[k] 
+        case app(f) => f.Map[x]
+        case orca(_, _) => Addr.ERR
+    case LP(zero, x) => 
+        match c.actors[a].st 
+        //add wf of frames?
+        case exe(f) => if x in f.Map then f.Map[x] else Addr.ERR
+        case snd(_, _, _, _) => Addr.ERR
+        case idl => Addr.ERR
+        case mkU(_) => Addr.ERR
+        case trc(_) => Addr.ERR
+        case mkR(_) => Addr.ERR
+        case cll(_) => Addr.ERR
+}
 
+
+lemma MP_wf(a: Actor, k: int) 
+ensures 0 <= k < |a.q| 
+
+//can we assume this?
+lemma all_actors_in_config()
+ensures forall a: ActorAddr, c: Config :: a in c.actors
+
+function method valid_addr(l: Addr) : bool {
+    true
+}
+
+function method C(a: ActorAddr, dp: DP, c: Config) : Addr 
+{
+    all_actors_in_config();
+    match dp 
+    case This => AA(a)
+    case MP(k, x) =>
+        MP_wf(c.actors[a], k);
+        CMP(k, x, c, c.actors[a]) 
+    case LP(zero, x) =>
+        CLP(zero, x, c, c.actors[a]) 
+    case cons(p, f) => 
+        assume C(a, p, c) in c.heap.objs;
+        var obj := c.heap.objs[C(a, p, c)];
+        if f in obj then obj[f] else Addr.ERR
+}
+function method CLP(zero: int, x: VarId, c: Config, a: Actor) : Addr
+{   
+    match a.st 
+    //add wf of frames?
+    case exe(f) => if x in f.Map then f.Map[x] else Addr.ERR
+    case snd(_, _, _, _) => Addr.ERR
+    case idl => Addr.ERR
+    case mkU(_) => Addr.ERR
+    case trc(_) => Addr.ERR
+    case mkR(_) => Addr.ERR
+    case cll(_) => Addr.ERR
+}
+
+function method CMP(k: int, x: VarId, c: Config, a: Actor) : Addr
+requires 0 <= k < |a.q|
+{
+    assert 0 <= k < |a.q|;
+    match a.q[k] 
+    case app(f) => if x in f.Map then f.Map[x] else Addr.ERR
+    case orca(_, _) => Addr.ERR
+}
+*/
